theories/Observe.v
@@ -3,16 +3,31 @@ From ITree Require Export
 From HTTP Require Export
      Tcp.
 
-Variant observeE : Type -> Set :=
-  Observe__ToServer : observeE (packetT exp)
+Variant observeE : Type -> Type :=
+  Observe__ToServer : server_state exp -> observeE (packetT id)
 | Observe__ToClient : observeE (packetT id).
+
+Definition wrap_field (f : field_line id) : field_line exp :=
+  let 'Field n v := f in Field n (Exp__Const v).
+
+Definition wrap_response (r : http_response id) : http_response exp :=
+  let 'Response l f ob := r in
+  Response l (map wrap_field f) (Exp__Const <$> (ob : option message_body)).
+
+Definition wrap_payload : payloadT id -> payloadT exp :=
+  fmap wrap_response.
+
+Definition wrap_packet (pkt : packetT id) : packetT exp :=
+  let 'Packet s d p := pkt in
+  Packet s d (wrap_payload p).
 
 Variant decideE : Type -> Set :=
   Decide : decideE bool.
 
 Variant unifyE : Type -> Type :=
-  Unify__Fresh   : unifyE (exp message_body)
-| Unify__Payload : payloadT exp -> payloadT id -> unifyE unit.
+  Unify__FreshBody : unifyE (exp message_body)
+| Unify__FreshETag : unifyE (exp field_value)
+| Unify__Response  : http_response exp -> http_response id -> unifyE unit.
 
 Notation failureE := (exceptE string).
 
@@ -21,17 +36,21 @@ Class Is__oE E `{failureE -< E} `{nondetE -< E}
 Notation oE := (failureE +' nondetE +' decideE +' unifyE +' observeE).
 Instance oE_Is__oE : Is__oE oE. Defined.
 
-Definition dualize {E R} `{Is__oE E} (e : switchE R) : itree E R :=
-  match e in switchE R return _ R with
-  | Switch__In => trigger Observe__ToServer
-  | Switch__Out (Packet s0 d0 p0) =>
+Definition dualize {E R} `{Is__oE E} (e : netE R) : itree E R :=
+  match e in netE R return _ R with
+  | Net__In st => wrap_packet <$> embed Observe__ToServer st
+  | Net__Out (Packet s0 d0 p0) =>
     '(Packet s d p) <- trigger Observe__ToClient;;
     if (s =? s0) &&& (d =? d0)
-    then embed Unify__Payload p0 p
+    then match p0, p with
+         | inl _, _
+         | _, inl _ => throw "Expect response but observed request"
+         | inr r0, inr r => embed Unify__Response r0 r
+         end
     else throw "Unexpected payload observed to client"
   end.
 
-Definition observer {E R} `{Is__oE E} (m : itree sE R) : itree E R :=
+Definition observer {E R} `{Is__oE E} (m : itree nE R) : itree E R :=
   interp
     (fun _ e =>
        match e with
@@ -42,6 +61,7 @@ Definition observer {E R} `{Is__oE E} (m : itree sE R) : itree E R :=
          end
        | (||se) =>
          match se in symE _ R return _ R with
-         | Sym__New => trigger Unify__Fresh
+         | Sym__NewBody => trigger Unify__FreshBody
+         | Sym__NewETag => trigger Unify__FreshETag
          end
        end) m.
