theories/Printer.v
@@ -1,4 +1,4 @@
-From Coq Require Export
+From Coq Require Import
      Ascii
      NArith
      String
