theories/Semantics.v
@@ -23,8 +23,10 @@ Open Scope list_scope.
 Open Scope monad_scope.
 Open Scope program_scope.
 
+Notation "P '?'" := (decide P) (at level 100).
+
 Program Instance Decidable_not {P} `{Decidable P} : Decidable (~ P) := {
-  Decidable_witness := negb Decidable_witness
+  Decidable_witness := negb (P?)
 }.
 Next Obligation.
   split; intro.
@@ -33,13 +35,17 @@ Next Obligation.
   - erewrite Decidable_sound_alt; intuition.
 Qed.
 
+Program Instance Decidable_eq_N (x y : N) : Decidable (x = y) :=
+  { Decidable_witness := N.eqb    x y;
+    Decidable_spec    := N.eqb_eq x y }.
+
 Program Instance Decidable_eq_list {A} `{forall x y : A, Decidable (x = y)}
         (x y : list A) : Decidable (x = y) := {
   Decidable_witness :=
     (fix eqb (x y : list A) :=
        match x, y with
        | [], [] => true
-       | a::x', b::y' => @Decidable_witness (a = b) _ &&& eqb x' y'
+       | a::x', b::y' => (a = b?) &&& eqb x' y'
        | _, _ => false
        end) x y }.
 Solve Obligations with split; intros; intro; intuition; discriminate.
@@ -61,32 +67,44 @@ Qed.
 Definition status_line_of_code (c : status_code) : status_line :=
   Status (Version 1 1) c (snd <$> find (N.eqb c ∘ fst) statusCodes).
 
-Definition server_state {exp_} := list (path * option (exp_ message_body)).
+Record resource_state exp_ :=
+  ResourceState {
+      resource__body : exp_ message_body;
+      resource__etag : option (exp_ field_value)
+    }.
+Arguments ResourceState {_}.
 
-Definition get {exp_} (p : path) : @server_state exp_ -> option (option (exp_ message_body)) :=
-  fmap snd ∘ find ((fun pq => decide (p = fst pq))).
+Definition server_state exp_ := list (path * option (resource_state exp_)).
 
-Definition put {exp_} : path -> option (exp_ message_body) -> server_state -> server_state
-  := compose cons ∘ pair.
+Definition get {K V} `{forall x y : K, Decidable (x = y)} (k : K) :
+  list (K * V) -> option V :=
+  fmap snd ∘ find ((fun kv => k = fst kv?)).
 
-Definition delete {exp_} (p : path) : @server_state exp_ -> server_state :=
-  filter (fun pq => (decide (p <> fst pq))).
+Definition delete {K V} `{forall x y : K, Decidable (x <> y)} (k : K) :
+  list (K * V) -> list (K * V) :=
+  filter (fun kv => (k <> fst kv?)).
 
-Notation var := nat.
+Definition put {K V} : K -> V -> list (K * V) -> list (K * V) :=
+  compose cons ∘ pair.
+
+Notation var := N.
 
 Inductive exp : Type -> Set :=
   Exp__Const : message_body -> exp message_body
-| Exp__Var   : var -> exp message_body.
+| Exp__Body  : var -> exp message_body
+| Exp__ETag  : var -> exp field_value
+| Exp__Match : field_value -> exp field_value -> exp bool.
 
 Notation connT := nat.
 
 Variant appE {exp_} : Type -> Type :=
-  App__Recv : appE (connT * http_request)
+  App__Recv : server_state exp_ -> appE (connT * http_request)
 | App__Send : connT -> http_response exp_ -> appE unit.
 Arguments appE : clear implicits.
 
 Variant symE {exp_} : Type -> Set :=
-  Sym__New : symE (exp_ message_body).
+  Sym__NewBody : symE (exp_ message_body)
+| Sym__NewETag : symE (exp_ field_value).
 Arguments symE : clear implicits.
 
 Class Is__smE E `{appE exp -< E} `{nondetE -< E} `{symE exp -< E}.
@@ -95,8 +113,8 @@ Instance smE_Is__smE : Is__smE smE. Defined.
 
 Definition http_smi {E R} `{Is__smE E} : itree E R :=
   rec
-    (fun st : @server_state exp =>
-       '(c, Request (RequestLine methd t _) hs om) <- trigger App__Recv;;
+    (fun st : server_state exp =>
+       '(c, Request (RequestLine methd t _) hs om) <- embed App__Recv st;;
        let bad_request :=
            trigger (App__Send c (Response (status_line_of_code 400) [] None));;
            call st in
@@ -112,17 +130,19 @@ Definition http_smi {E R} `{Is__smE E} : itree E R :=
                trigger (App__Send c (@Response exp (status_line_of_code 200)
                                              [] (Some m))) in
            match get p st with
-           | Some (Some m) => ok m;; call st
+           | Some (Some (ResourceState m _)) => ok m;; call st
            | Some None => not_found;; call st
            | None =>
-             or (not_found;; call ((p, None)::st))
-                (m <- trigger (@Sym__New exp);; ok m;; call ((p, Some m)::st))
+             or (not_found;; call (put p None st))
+                (mx <- trigger (@Sym__NewBody exp);;
+                 ok mx;;
+                 call (put p (Some (ResourceState mx None)) st))
            end
          | Method__PUT =>
            match om with
            | Some m =>
              trigger (App__Send c (Response (status_line_of_code 204) [] None));;
-             call (put p (Some (Exp__Const m)) $ delete p st)
+             call (put p (Some (ResourceState (Exp__Const m) None)) st)
            | None => bad_request
            end
          | _ =>
