theories/Tester.v
@@ -1,0 +1,170 @@
+From ExtLib Require Export
+     OptionMonad.
+From HTTP Require Export
+     Printer
+     Observe.
+Open Scope N_scope.
+Open Scope string_scope.
+
+Definition exp_state : Set := list (var * option message_body) *
+                              list (var * (field_value + list field_value)).
+
+Definition fresh_var {T} (vs : list (var * T)) : var :=
+  1 + fold_left N.max (map fst vs) 0.
+
+Definition fresh_body (s : exp_state) : exp_state * var :=
+  let (bs, es) := s in
+  let x := fresh_var bs in
+  ((x, None) :: bs, es, x).
+
+Definition fresh_etag (s : exp_state) : exp_state * var :=
+  let (bs, es) := s in
+  let x := fresh_var es in
+  (bs, (x, inr []) :: es, x).
+
+Definition assert (x : var) (v : field_value) (s : exp_state)
+  : option exp_state :=
+  let (bs, es) := s in
+  match get x es with
+  | Some (inl e)  => if e =? v then Some s else None
+  | Some (inr ts) => if existsb (eqb v) ts
+                    then None
+                    else Some (bs, put x (inl v) es)
+  | None => Some (bs, put x (inl v) es)
+  end.
+
+Definition assert_not (x : var) (v : field_value) (s : exp_state)
+  : option exp_state :=
+  let (bs, es) := s in
+  match get x es with
+  | Some (inl e) => if e =? v then None else Some s
+  | Some (inr ts) => Some (bs, put x (inr (v :: ts)) es)
+  | None          => Some (bs, put x (inr [v]) es)
+  end.
+
+Definition unify {T} (e : exp T) (v : T) (s : exp_state) : option exp_state :=
+  match e in exp T return T -> exp_state -> option exp_state with
+  | Exp__Const m => fun v s => if m =? v then Some s else None
+  | Exp__Body x =>
+    fun v s =>
+      let (bs, es) := s in
+      match get x bs with
+      | Some (Some b) => if b =? v then Some s else None
+      | Some None     => None
+      | None          => Some (put x (Some v) bs, es)
+      end
+  | Exp__ETag x => assert x
+  | Exp__Match f (Exp__ETag x) =>
+    fun v => if v then assert x f else assert_not x f
+  | Exp__Match _ _ => fun _ _ => None
+  end v s.
+
+Variant genE : Type -> Type :=
+  Gen : server_state exp -> exp_state -> genE (packetT id).
+
+Variant clientE : Type -> Type :=
+  Client__Recv : clientE (packetT id)
+| Client__Send : packetT id -> clientE unit.
+
+Class Is__tE E `{failureE -< E} `{nondetE -< E} `{genE -< E} `{clientE -< E}.
+Notation tE := (failureE +' nondetE +' genE +' clientE).
+Instance tE_Is__tE : Is__tE tE. Defined.
+
+CoFixpoint match_event {T R} (e0 : observeE R) (r : R) (m : itree oE T)
+  : itree oE T :=
+  match observe m with
+  | RetF x  => Ret x
+  | TauF m' => Tau (match_event e0 r m')
+  | VisF e k =>
+    match e with
+    | (||||oe) =>
+      match oe in observeE Y, e0 in observeE R return (Y -> _) -> R -> _ with
+      | Observe__ToServer _, Observe__ToServer _
+      | Observe__ToClient, Observe__ToClient => id
+      | _, _ => fun _ _ => throw "Unexpected event"
+      end k r
+    | _ => vis e (match_event e0 r ∘ k)
+    end
+  end.
+
+Definition match_observe {T R} (e : observeE T) (r : T) (l : list (itree oE R))
+  : list (itree oE R) := map (match_event e r) l.
+
+CoFixpoint tester' {E R} `{Is__tE E} (s : exp_state) (others : list (itree oE R))
+           (m : itree oE R) : itree E R :=
+  match observe m with
+  | RetF r => Ret r
+  | TauF m' => Tau (tester' s others m')
+  | VisF e k =>
+    let catch (err : string) : itree E R :=
+        match others with
+        | [] => throw err
+        | other :: others' => Tau (tester' s others' other)
+        end in
+    match e with
+    | (Throw err|) => catch err
+    | (|ne|) =>
+      match ne in nondetE Y return (Y -> _) -> _ with
+      | Or => fun k => b <- trigger Or;; Tau (tester' s others (k b))
+      end k
+    | (||de|) =>
+      match de in decideE Y return (Y -> _) -> _ with
+      | Decide => fun k => b <- trigger Or;;
+                       Tau (tester' s (k (negb b) :: others) (k b))
+      end k
+    | (|||ue|) =>
+      match ue in unifyE Y return (Y -> _) -> _ with
+      | Unify__FreshBody => fun k => let (s', x) := fresh_body s in
+                               Tau (tester' s' others (k (Exp__Body x)))
+      | Unify__FreshETag => fun k => let (s', x) := fresh_etag s in
+                               Tau (tester' s' others (k (Exp__ETag x)))
+      | Unify__Response rx r =>
+        fun k =>
+          let 'Response (Status _ cx _ as stx) fx obx := rx in
+          let 'Response (Status _ c  _ as st ) fs ob  := r  in
+          if cx = c?
+          then
+            let unify_field (os : option exp_state) (f : field_line exp)
+                : option exp_state :=
+                match os with
+                | Some s =>
+                  let 'Field n vx := f in
+                  match field__value <$> find (eqb n ∘ field__name) fs with
+                  | Some v => unify vx (v : id field_value) s
+                  | None   => None
+                  end
+                | None => None
+                end in
+            let os1 : option exp_state := fold_left unify_field fx (Some s) in
+            match os1 with
+            | Some s1 =>
+              match obx, ob with
+              | Some bx, Some b =>
+                match unify bx b s1 with
+                | Some s2 => Tau (tester' s2 others (k tt))
+                | None    => catch "Message body unsatisfying."
+                end
+              | Some _, None => catch "Expect message body, but not found."
+              | None, Some _ => catch "Expect no message body, but observed it."
+              | None, None => Tau (tester' s1 others (k tt))
+              end
+            | None => catch "Field lines unsatisfying."
+            end
+          else catch $ "Expect status " ++ status_to_string stx
+                    ++ " but observed " ++ status_to_string st
+      end k
+    | (||||oe) =>
+      match oe in observeE Y return (Y -> _) -> _ with
+      | Observe__ToServer st =>
+        fun k => pkt <- embed Gen st s;;
+              embed Client__Send pkt;;
+              Tau (tester' s (match_observe (Observe__ToServer st) pkt others) (k pkt))
+      | Observe__ToClient =>
+        fun k => pkt <- trigger Client__Recv;;
+              Tau (tester' s (match_observe Observe__ToClient pkt others) (k pkt))
+      end k
+    end
+  end.
+
+Definition tester {E R} `{Is__tE E} : itree oE R -> itree E R :=
+  tester' ([], []) [].
